src/langs/STLC.v
@@ -117,3 +117,331 @@ Proof using.
   Unshelve.
     all: solve [ exact (con 0 [::]) | exact [::]].
 Qed.
+(*
+Notation bot g := (con 30 [::g]).
+Definition tgt :=
+  (term_rule [:: ob] (ty 0))::stlc.
+
+Lemma wf_tgt : wf_lang tgt.
+Proof using .
+  constructor.
+  apply stlc_wf.
+  constructor; eauto with judgment.
+  econstructor; eauto with judgment.
+  ltac2:(unify_nth_level ()).
+  constructor; eauto with judgment.
+  econstructor; eauto with judgment.
+  by cbv.
+  Unshelve.
+  all: solve [exact (con 0 [::]) | exact [::]].
+Qed.
+*)
+From excomp Require Import Compilers.
+
+Notation "'cfun' pat => e" :=
+  (fun s =>
+     match s with
+     | pat => e
+     | _ => con 0 [::]
+     end)
+    (at level 60, pat pattern).
+
+(*
+Definition cps : compiler :=
+  [:: (*TODO*)
+     (cfun [:: f; g; a; b; c] =>
+        (cmp a b c f g)
+     );
+  (fun s =>
+     let withK g := (ext g (bot g)) in
+     (con 1 (map withK s)));
+  (fun s => con 0 s)].
+*)
+
+Notation dyn g := (con 27 [:: g]%exp_scope).
+Notation dlam g e := (con 29 [:: e; g]%exp_scope).
+Notation dapp g e e' := (con 30 [:: e'; e; g]%exp_scope).
+
+Notation dpair g e1 e2 := (con 32 [:: e2; e1; g]%exp_scope).
+Notation dproj1 g e := (con 33 [:: e; g]%exp_scope).
+Notation dproj2 g e := (con 34 [:: e; g]%exp_scope).
+
+Notation unit g := (con 37 [:: g]%exp_scope).
+Definition cc :=
+  (term_rule [:: ob] (el 0 (dyn 0)))::
+  (term_le [:: el 0 (dyn 0);
+             el 0 (dyn 0);
+             ob]
+           (dproj2 0 (dpair 0 1 2))
+           2
+           (el 0 (dyn 0)))::
+  (term_le [:: el 0 (dyn 0);
+             el 0 (dyn 0);
+             ob]
+           (dproj1 0 (dpair 0 1 2))
+           1
+           (el 0 (dyn 0)))::
+  (term_rule [:: el 0 (dyn 0); ob] (el 0 (dyn 0)))::
+  (term_rule [:: el 0 (dyn 0); ob] (el 0 (dyn 0)))::
+  (term_rule [:: el 0 (dyn 0);
+             el 0 (dyn 0);
+             ob]
+             (el 0 (dyn 0)))::
+  (term_le [:: el 0 (dyn 0);
+               el (ext emp (dyn emp)) (dyn (ext emp (dyn emp))); ob]
+           (dapp 0 (dlam 0 1) 2)
+           (el_subst 0 (ext emp (dyn emp))
+                     (snoc 0 emp (dyn emp) (forget 0) 2)
+                     (dyn (ext emp (dyn emp))) 1)
+           (el 0 (dyn 0)))::
+  (term_rule [:: el 0 (dyn 0); el 0 (dyn 0); ob]
+             (el 0 (dyn 0)))::
+  (term_rule [:: el (ext emp (dyn emp)) (dyn (ext emp (dyn emp))); ob]
+             (el 0 (dyn 0)))::
+  (term_le [:: hom 0 1; ob; ob]
+           (ty_subst 0 1 2 (dyn 1))
+           (dyn 0)
+           (ty 0))::
+  (term_rule [:: ob] (ty 0))::
+  subst_lang.
+
+Lemma cc_wf : wf_lang cc.
+Proof.
+  pose swf := subst_lang_wf.
+  wf_lang_eauto.
+  2: by cbv.
+   {
+    constructor; eauto with judgment.
+    eapply wf_term_conv.
+    eauto with judgment.
+    ltac2:(apply_term_constr ()).
+    eapply wf_subst_cons; eauto with judgment.
+    eapply wf_subst_cons; eauto with judgment.
+    eapply wf_subst_cons; eauto with judgment.
+    {
+      cbv.
+      ltac2:(apply_term_constr()).
+      eapply wf_subst_cons; eauto with judgment.
+      cbv.
+      eapply wf_term_conv.
+      eauto with judgment.
+      eapply wf_term_var.
+      ltac2:(unify_nth_level()).
+      eapply sort_con_mor.
+      eapply subst_cons_mor.
+      eauto with judgment.
+      symmetry.
+      instantiate (1 := ty 0).
+      cbv.
+      ltac2:(apply_term_rule constr:(28)).
+      eauto with judgment.      
+    }
+    {
+      cbv.
+      eapply sort_con_mor.
+      eapply le_subst_cons.
+      eauto with judgment.
+      instantiate (1:= ty 0).
+      cbv.
+      ltac2:(apply_term_rule constr:(28)).
+      repeat (eapply le_subst_cons; eauto with judgment).
+    }
+   }
+Unshelve.
+    all: solve [ exact (con 0 [::]) | exact [::]].
+Qed.
+
+Definition dummy := (fun s : subst => con 0 [::]).
+Definition subst_id_comp : compiler :=
+  [::
+     dummy;
+  dummy;
+  dummy;
+  dummy;
+  con 22;
+  con 21;
+  con 20;
+  con 19;
+  dummy;
+  dummy;
+  con 16;
+  con 15;
+  dummy;
+  dummy;
+  dummy;
+  dummy;
+  con 10;
+  con 9;
+  con 8;
+  con 7;
+  dummy;
+  dummy;
+  dummy;
+  con 3;
+  con 2;
+  con 1;
+  con 0].
+
+Print ("f":string).
+
+Lemma subst_id_comp_preserves : preserving_compiler cc subst_id_comp subst_lang.
+Proof.
+  eapply preserving_compiler_term_le.
+  2:{
+    intro s.
+    simpl.
+    change (nth_level (fun=> ob) _ ?n) with (con n).
+    inversion; subst.
+    inversion H2; subst.
+    inversion H3; subst.
+    move: H5 H8.
+    clear H3 H7 H2 H H4.
+    change (var_lookup [:: e; e0] 0) with e0. 
+    change (var_lookup [:: e; e0] 1) with e.
+    intros.
+    change (le_term cc [::] (hom (ext e0 e) (ext e0 e)) (id (ext e0 e))
+    (snoc (ext e0 e) e0 e (p e0 e) (q e0 e))) with
+        (le_term cc [::]
+                 (hom (ext 0 1) (ext 0 1))[/[:: e; e0]/]
+                 (id (ext 0 1))[/[:: e; e0]/]
+                 (snoc (ext 0 1) 0 1 (p 0 1) (q 0 1))[/[:: e;e0]/]).
+    eapply le_term_subst.
+    2:{
+      eapply le_term_by.
+      by instantiate (1:= [:: ty 0; ob]).
+    }
+    {
+      eauto with judgment.
+    }
+  }
+  eapply preserving_compiler_term_le.
+  eapply preserving_compiler_term_le.
+  eapply preserving_compiler_term_le.
+  eapply preserving_compiler_term.
+  2:{
+    intro s.
+    simpl.
+    change (nth_level (fun=> ob) _ ?n) with (con n).
+    inversion; subst.
+    inversion H2; subst.
+    inversion H3; subst.
+    change (var_lookup [:: e; e0] 0) with e0. 
+    change (var_lookup [:: e; e0] 1) with e.
+    ltac2:(apply_term_constr ()).
+    econstructor; eauto with judgment.
+    eapply wf_sort_by.
+    ltac2:(unify_nth_level()).
+    constructor; eauto with judgment.
+    move: H5.
+    change (var_lookup [:: e; e0] 0) with e0.
+    change (ty 0)[/[::e0]/] with (ty e0).
+    replace  (ty e0) [/[:: e0] /] with (ty e0); auto.
+    unfold exp_subst.
+    simpl.
+    f_equal.
+    f_equal.
+    give_up(* TODO: lemma about closed terms*).
+  }
+  
+  eapply preserving_compiler_term.
+  eapply preserving_compiler_term.
+  eapply preserving_compiler_term.
+  eapply preserving_compiler_term_le.
+  eapply preserving_compiler_term_le.
+  eapply preserving_compiler_term.
+  eapply preserving_compiler_term.
+  eapply preserving_compiler_term_le.
+  eapply preserving_compiler_term_le.
+  eapply preserving_compiler_term_le.
+  eapply preserving_compiler_term_le.
+  eapply preserving_compiler_term.
+  eapply preserving_compiler_sort.
+  eapply preserving_compiler_term.
+  eapply preserving_compiler_sort.
+  eapply preserving_compiler_term_le.
+  eapply preserving_compiler_term_le.
+  eapply preserving_compiler_term_le.
+  eapply preserving_compiler_term.
+  eapply preserving_compiler_term.
+  eapply preserving_compiler_sort.
+  eapply preserving_compiler_sort.
+  eapply preserving_compiler_nil.
+Admitted.
+
+Definition dweaken g t e :=
+  el_subst (ext g t) g (p g t) (dyn g) e.
+Fixpoint mkenv_tuple g : exp :=
+  match g with
+  | emp => (unit emp)
+  | ext g' t => (dpair (ext g' t) (q g' t) (dweaken g' t (mkenv_tuple g')))
+  | _ => con 0 [::]
+  end.
+
+Fixpoint mkenv_subst g pr : exp :=
+  match g with
+  | emp => id emp
+  | ext g' t =>
+    let ge := ext emp (dyn emp) in
+    snoc ge g' t
+         (mkenv_subst g' (dproj2 ge pr))
+         (dproj1 ge pr)
+  | _ => con 0 [::]
+  end.
+
+Definition compile_arr :=
+  cfun [:: b; a; g] => dyn g.
+
+Definition compile_abstr :=
+ cfun [:: g; a; b; e] =>
+   dpair g (dlam g (el_subst (ext emp (dyn emp))
+                             (ext g a)
+                             (mkenv_subst g (q emp (dyn emp)))
+                             (dyn (ext g a)) e))
+         (mkenv_tuple g). 
+
+Definition cc_comp : compiler :=
+  [:: dummy;
+  dummy;
+  compile_abstr;
+  compile_arr
+  ]++ subst_id_comp.
+
+Lemma cc_comp_preserves
+  : preserving_compiler cc cc_comp stlc.
+Proof.
+  eapply preserving_compiler_term_le.
+  eapply preserving_compiler_term.
+  eapply preserving_compiler_term.
+  eapply preserving_compiler_term.
+  apply subst_id_comp_preserves.
+  {
+    intro s.
+    simpl.
+    change (nth_level (fun=> ob) _ ?n) with (con n).
+    inversion;subst.
+    inversion H2; subst.
+    inversion H3; subst.
+    inversion H6; subst.
+    change (var_lookup _ 0) with e1.
+    cbv.
+    ltac2:(apply_term_constr()).
+    constructor; eauto with judgment.
+  }
+  {
+    intro s; simpl.               
+    change (nth_level (fun=> ob) _ 27) with compile_arr.
+    change (nth_level (fun=> ob) _ ?n) with (con n).
+    inversion;subst.
+    inversion H2; subst.
+    inversion H3; subst.
+    inversion H6; subst.
+    inversion H9; subst.
+    move: H5.
+    change (var_lookup _ 0) with e2.
+    change (var_lookup _ 1) with e1.
+    change (var_lookup _ 2) with e0.
+    unfold compile_arr.
+    unfold compile_abstr.
+    intro.
+    ltac2:(apply_term_constr()).
+    constructor; eauto with judgment.
